typeclass_env_map: add some entail theorems

typeclass/typeclass_env_map_implScript.sml
@@ -4,9 +4,10 @@ open HolKernel Parse boolLib bossLib dep_rewrite BasicProvers;
 open relationTheory set_relationTheory;
 open pairTheory optionTheory listTheory pred_setTheory finite_mapTheory;
 open mlmapTheory mlstringTheory balanced_mapTheory alistTheory topological_sortTheory;
-open miscTheory typeclass_unificationTheory
+open miscTheory typeclass_unificationTheory typeclass_typesTheory
   typeclass_inference_commonTheory typeclass_tcexpTheory
   typeclass_specializeTheory;
+open monadsyntax;
 
 val _ = new_theory "typeclass_env_map_impl";
 
@@ -155,6 +156,13 @@ Proof
   simp[ty_args_def,ty_args_aux_SNOC]
 QED
 
+Theorem ty_args_alt:
+  (∀t1 t2. ty_args (Cons t1 t2) = SNOC t2 (ty_args t1)) ∧
+  (∀x. ty_args (Atom x) = [])
+Proof
+  simp[ty_args_SNOC] >> simp[ty_args_def,ty_args_aux_def]
+QED
+
 Definition split_ty_head_aux_def:
   split_ty_head_aux (Cons t1 t2) l = split_ty_head_aux t1 (t2::l) ∧
   split_ty_head_aux (Atom $ TypeCons tc) l = SOME (tc,l) ∧
@@ -175,7 +183,7 @@ Definition split_ty_head_def:
 End
 
 Theorem split_ty_head_thm:
-  ∀t tc targs. 
+  ∀t tc targs.
     split_ty_head t = SOME (tc,targs) ⇔
     (head_ty_cons t = SOME tc ∧ ty_args t = targs)
 Proof
@@ -417,7 +425,7 @@ Proof
     ) >>
     rw[MEM_MAP] >>
     `{s | super_reachable (to_class_map cl_map) c s ∨ c = s} =
-    {s | super_reachable (to_class_map cl_map) c s} ∪ {c}` 
+    {s | super_reachable (to_class_map cl_map) c s} ∪ {c}`
       by (
         rw[EXTENSION] >>
         metis_tac[]
@@ -456,7 +464,7 @@ Definition by_super_aux_def:
       | NONE => NONE
       | SOME clinfo =>
           by_super_aux_list cl_map (insert visited c t) clinfo.super t
-   else NONE) ∧ 
+   else NONE) ∧
   by_super_aux_list cl_map ret [] t = SOME ret ∧
   by_super_aux_list cl_map visited (sup::xs) t =
     if map_ok cl_map ∧ map_ok visited
@@ -1039,22 +1047,26 @@ Proof
   metis_tac[]
 QED
 
+(* every class in the super list must be a valid key of the map *)
+Definition super_keys_ok_def:
+  super_keys_ok cl_map =
+  (∀c clinfo c'.
+    mlmap$lookup cl_map c = SOME clinfo ∧ MEM c' clinfo.super ⇒
+    ∃x. mlmap$lookup cl_map c' = SOME x)
+End
+
 (* everything in the super list must be in the map *)
 Theorem well_formed_by_super_aux:
   (∀cl_map visited c (t:'a) clinfo.
     map_ok cl_map ∧ map_ok visited ∧
-    (∀c clinfo c'.
-      mlmap$lookup cl_map c = SOME clinfo ∧ MEM c' clinfo.super ⇒
-      ∃x. mlmap$lookup cl_map c' = SOME x) ⇒
+    super_keys_ok cl_map ⇒
     ((∃clinfo. mlmap$lookup cl_map c = SOME clinfo ∨
       (∃m. lookup visited c = SOME m)) ⇔
     (∃m. by_super_aux cl_map visited c t = SOME m))) ∧
 
   ∀cl_map visited cs (t:'a).
     map_ok cl_map ∧ map_ok visited ∧
-    (∀c clinfo c'.
-      mlmap$lookup cl_map c = SOME clinfo ∧ MEM c' clinfo.super ⇒
-      ∃x. mlmap$lookup cl_map c' = SOME x) ⇒
+    super_keys_ok cl_map ⇒
     ((∀c. MEM c cs ⇒
       (∃clinfo. mlmap$lookup cl_map c = SOME clinfo ∨
       (∃m. lookup visited c = SOME m))) ⇔
@@ -1071,11 +1083,11 @@ Proof
       rpt TOP_CASE_TAC
     ) >>
     rpt TOP_CASE_TAC >> gvs[] >>
-    metis_tac[]
+    metis_tac[super_keys_ok_def]
   ) >>
   rw[Once full_by_super_aux_def] >>
   TOP_CASE_TAC >>
-  gvs[] >- metis_tac[] >>
+  gvs[super_keys_ok_def] >- metis_tac[] >>
   rename1`by_super_aux cl_map visited c t = SOME x` >>
   `map_ok x` by metis_tac[cj 1 $ cj 1 by_super_aux_monotone] >>
   iff_tac
@@ -1146,10 +1158,7 @@ QED
 
 Theorem well_formed_by_super:
   ∀cl_map c (t:'a) clinfo.
-    map_ok cl_map ∧
-    (∀c clinfo c'.
-      mlmap$lookup cl_map c = SOME clinfo ∧ MEM c' clinfo.super ⇒
-      ∃x. mlmap$lookup cl_map c' = SOME x) ⇒
+    map_ok cl_map ∧ super_keys_ok cl_map ⇒
     ((∃clinfo. mlmap$lookup cl_map c = SOME clinfo) ⇔
     (∃m. by_super cl_map (c,t) = SOME m))
 Proof
@@ -1163,20 +1172,51 @@ QED
 
 Definition lookup_inst_map_def:
   lookup_inst_map inst_map c t =
-    OPTION_BIND (split_ty_head t) (λ(tcons,targs).
-      OPTION_BIND (lookup inst_map (c,tcons)) (λinst_info.
-      if LENGTH targs = inst_info.nargs
-      then
-        SOME $ (inst_info.impl, MAP (I ## flip EL targs) inst_info.cstr)
-      else NONE))
+  do
+    (tcons,targs) <- split_ty_head t;
+    inst_info <- lookup inst_map (c,tcons);
+    assert (LENGTH targs = inst_info.nargs);
+    return (inst_info.impl, MAP (I ## flip EL targs) inst_info.cstr)
+  od
 End
 
 Definition by_inst_def:
   by_inst inst_map c t = OPTION_MAP SND $ lookup_inst_map inst_map c t
 End
 
+Theorem lookup_inst_map_lem:
+  ∀inst_map c t impl cstr.
+    lookup_inst_map inst_map c t = SOME (impl,cstr)
+    ⇔
+    (∃tcons targs inst_info.
+      split_ty_head t = SOME (tcons,targs) ∧
+      lookup inst_map (c,tcons) = SOME inst_info ∧
+      LENGTH targs = inst_info.nargs ∧
+      impl = inst_info.impl ∧
+      cstr = MAP (I ## (λv. EL v targs)) inst_info.cstr)
+Proof
+  reverse $ rw[lookup_inst_map_def,EQ_IMP_THM]
+  >- simp[combinTheory.C_DEF] >>
+  pairarg_tac >>
+  gvs[combinTheory.C_DEF]
+QED
+
+Theorem by_inst_lem:
+  ∀inst_map c t cstr.
+  by_inst inst_map c t = SOME cstr ⇔
+  (∃tcons targs inst_info.
+    split_ty_head t = SOME (tcons,targs) ∧
+    lookup inst_map (c,tcons) = SOME inst_info ∧
+    LENGTH targs = inst_info.nargs ∧
+      cstr = MAP (I ## (λv. EL v targs)) inst_info.cstr)
+Proof
+  simp[by_inst_def,LAMBDA_PROD,GSYM PEXISTS_THM,lookup_inst_map_lem]
+QED
+
 Theorem lookup_inst_map_thm:
   ∀inst_map c t impl cstr.
+    lookup_inst_map inst_map c t = SOME (impl,cstr)
+    ⇔
     (∃tcons targs inst_info.
       split_ty_head t = SOME (tcons,targs) ∧
       lookup inst_map (c,tcons) = SOME inst_info ∧
@@ -1186,10 +1226,8 @@ Theorem lookup_inst_map_thm:
       (∀n. n < LENGTH inst_info.cstr ⇒
         let (cl,v) = EL n inst_info.cstr in
           EL n cstr = (cl,EL v targs)))
-    ⇔
-    lookup_inst_map inst_map c t = SOME (impl,cstr)
 Proof
-  rw[lookup_inst_map_def,EQ_IMP_THM]
+  reverse $ rw[lookup_inst_map_lem,EQ_IMP_THM]
   >- (
     simp[] >>
     irule LIST_EQ >>
@@ -1198,8 +1236,6 @@ Proof
     first_x_assum drule >>
     simp[]
   ) >>
-  pairarg_tac >>
-  gvs[] >>
   rw[] >>
   pairarg_tac >>
   gvs[EL_MAP,oneline PAIR_MAP_THM]
@@ -1207,6 +1243,7 @@ QED
 
 Theorem by_inst_thm:
   ∀inst_map c t cstr.
+    by_inst inst_map c t = SOME cstr ⇔
     (∃tcons targs inst_info.
       split_ty_head t = SOME (tcons,targs) ∧
       lookup inst_map (c,tcons) = SOME inst_info ∧
@@ -1215,10 +1252,8 @@ Theorem by_inst_thm:
       (∀n. n < LENGTH inst_info.cstr ⇒
         let (cl,v) = EL n inst_info.cstr in
           EL n cstr = (cl,EL v targs)))
-    ⇔
-    by_inst inst_map c t = SOME cstr
 Proof
-  simp[by_inst_def,LAMBDA_PROD,GSYM PEXISTS_THM,GSYM lookup_inst_map_thm]
+  simp[by_inst_def,LAMBDA_PROD,GSYM PEXISTS_THM,lookup_inst_map_thm]
 QED
 
 Inductive full_entail:
@@ -1247,12 +1282,31 @@ Inductive entail:
   entail cl_map inst_map ps (c,t)
 End
 
-(*
+Theorem split_ty_head_tsubst:
+  ∀t tcons targs ts.
+    split_ty_head t = SOME (tcons,targs) ⇒
+    split_ty_head (tsubst ts t) = SOME (tcons, MAP (tsubst ts) targs)
+Proof
+  ho_match_mp_tac head_ty_cons_ind >>
+  rw[] >>
+  gvs[subst_db_def,split_ty_head_thm,head_ty_cons_def,ty_args_alt]
+QED
+
+Definition well_scoped_inst_map_def:
+  well_scoped_inst_map inst_map =
+  (∀k inst_info c v.
+    lookup inst_map k = SOME inst_info ∧
+    MEM (c,v) inst_info.cstr ⇒
+    v < inst_info.nargs)
+End
+
 Theorem entail_tsubst:
+  well_scoped_inst_map inst_map ⇒
   ∀p. entail cl_map inst_map ps p ⇒
   ∀c t ts. p = (c,t) ⇒
   entail cl_map inst_map (MAP (λ(c',t'). (c',tsubst ts t')) ps) (c,tsubst ts t)
 Proof
+  strip_tac >>
   ho_match_mp_tac entail_ind >>
   rw[]
   >- (
@@ -1276,11 +1330,172 @@ Proof
     pairarg_tac >>
     gvs[]
   ) >>
-  drule by_inst_SOME >>
+  gvs[by_inst_thm] >>
+  drule_then (irule_at (Pos hd)) split_ty_head_tsubst >>
   rw[] >>
-  irule EQ_TRANS >>
-  irule_at (Pos hd) $ cj 4 by_inst_thm >>
-  simp[]
+  first_x_assum drule >>
+  pairarg_tac >> gvs[EL_MAP] >>
+  DEP_REWRITE_TAC[EL_MAP] >>
+  gvs[well_scoped_inst_map_def] >>
+  last_x_assum irule >>
+  simp[MEM_EL] >>
+  metis_tac[]
+QED
+
+Theorem full_entail_tsubst:
+  well_scoped_inst_map inst_map ⇒
+  ∀p. full_entail cl_map inst_map ps p ⇒
+  ∀c t ts. p = (c,t) ⇒
+  full_entail cl_map inst_map (MAP (λ(c',t'). (c',tsubst ts t')) ps) (c,tsubst ts t)
+Proof
+  strip_tac >>
+  ho_match_mp_tac full_entail_ind >>
+  rw[]
+  >- (
+    irule full_entail_mem >>
+    simp[MEM_MAP] >>
+    first_x_assum $ irule_at (Pos last) >>
+    simp[]
+  )
+  >- (
+    irule full_entail_super >>
+    simp[MEM_MAP,PULL_EXISTS] >>
+    first_assum $ irule_at (Pos last) >>
+    first_assum $ irule_at (Pos last) >>
+    simp[]
+  ) >>
+  irule full_entail_inst >>
+  qexists `MAP (λ(c',t'). (c',tsubst ts t')) qs` >>
+  rw[MEM_MAP]
+  >- (
+    first_x_assum $ drule_then strip_assume_tac >>
+    pairarg_tac >>
+    gvs[]
+  ) >>
+  gvs[by_inst_thm] >>
+  drule_then (irule_at (Pos hd)) split_ty_head_tsubst >>
+  rw[] >>
+  first_x_assum drule >>
+  pairarg_tac >> gvs[EL_MAP] >>
+  DEP_REWRITE_TAC[EL_MAP] >>
+  gvs[well_scoped_inst_map_def] >>
+  last_x_assum irule >>
+  simp[MEM_EL] >>
+  metis_tac[]
+QED
+
+Definition cons_types_def:
+  cons_types thd [] = thd ∧
+  cons_types thd (t1::targs) = cons_types (Cons thd t1) targs
+End
+
+Definition tcons_to_type_def:
+  tcons_to_type tcons targs = cons_types (Atom $ TypeCons tcons) targs
+End
+
+Theorem head_ty_cons_cons_types:
+  ∀t targs. head_ty_cons (cons_types t targs) = head_ty_cons t
+Proof
+  Induct_on `targs` >>
+  rw[head_ty_cons_def,cons_types_def]
+QED
+
+Theorem ty_args_cons_types:
+  ∀t targs. ty_args (cons_types t targs) = ty_args t ++ targs
+Proof
+  Induct_on `targs` >>
+  rw[cons_types_def,ty_args_alt]
+QED
+
+Theorem tcons_to_type_alt:
+  (∀tcons. tcons_to_type tcons [] = Atom $ TypeCons tcons) ∧
+  (∀tcons t1 targs.
+    tcons_to_type tcons (t1::targs) =
+      cons_types (Cons (Atom $ TypeCons tcons) t1) targs)
+Proof
+  rw[tcons_to_type_def] >>
+  simp[Once cons_types_def]
+QED
+
+Theorem split_ty_head_tcons_to_type:
+  split_ty_head (tcons_to_type tcons targs) = SOME (tcons, targs)
+Proof
+  Induct_on `targs` using SNOC_INDUCT >>
+  gvs[tcons_to_type_def,split_ty_head_thm] >>
+  rw[cons_types_def,ty_args_alt,head_ty_cons_def] >>
+  gvs[head_ty_cons_cons_types,ty_args_cons_types]
+QED
+
+Theorem cons_types_APPEND:
+   ∀t ts1 ts2.
+     cons_types t (ts1 ++ ts2) = cons_types (cons_types t ts1) ts2
+Proof
+  Induct_on `ts1` >>
+  rw[cons_types_def]
+QED
+
+Theorem cons_types_SNOC:
+  ∀t ts1 t2. cons_types t (ts1 ++ [t2]) = Cons (cons_types t ts1) t2
+Proof
+  simp[cons_types_APPEND,cons_types_def]
+QED
+
+Theorem tcons_to_type_APPEND:
+  tcons_to_type tcons (ts1 ++ ts2) = cons_types (tcons_to_type tcons ts1) ts2
+Proof
+  simp[tcons_to_type_def,cons_types_APPEND]
+QED
+
+Theorem tcons_to_type_SNOC:
+  tcons_to_type tcons (SNOC t ts1) = Cons (tcons_to_type tcons ts1) t
+Proof
+  simp[tcons_to_type_APPEND,SNOC_APPEND,cons_types_def]
+QED
+
+Theorem tcons_to_type_split_ty_head:
+  ∀t tcons targs.
+    split_ty_head t = SOME (tcons,targs) ⇒
+    tcons_to_type tcons targs = t
+Proof
+  ho_match_mp_tac head_ty_cons_ind >>
+  rw[] >>
+  gvs[split_ty_head_thm,head_ty_cons_def,
+    ty_args_alt,tcons_to_type_alt] >>
+  gvs[tcons_to_type_def,cons_types_SNOC]
+QED
+
+Theorem tcons_to_type_NEQ_TypeVar:
+  ∀v. tcons_to_type tcons targs ≠ TypeVar v
+Proof
+  rpt strip_tac >>
+  pop_assum $ mp_tac o Q.AP_TERM `split_ty_head` >>
+  simp[split_ty_head_tcons_to_type,split_ty_head_thm,head_ty_cons_def]
+QED
+
+Theorem tsubst_cons_types:
+  ∀thd. tsubst ts (cons_types thd targs) =
+    cons_types (tsubst ts thd) $ MAP (tsubst ts) targs
+Proof
+  Induct_on `targs` >>
+  rw[cons_types_def,subst_db_def]
+QED
+
+Theorem tsubst_tcons_to_type:
+  tsubst ts (tcons_to_type tcons targs) =
+    tcons_to_type tcons $ MAP (tsubst ts) targs
+Proof
+  rw[tcons_to_type_def,tsubst_cons_types,subst_db_def]
+QED
+
+Triviality tcons_to_type_tsubst_TypeVar:
+  tcons_to_type tcons targs =
+    tsubst targs $ tcons_to_type tcons $ GENLIST TypeVar (LENGTH targs)
+Proof
+  simp[tsubst_tcons_to_type,MAP_GENLIST] >>
+  AP_TERM_TAC >>
+  PURE_REWRITE_TAC[Once $ GSYM GENLIST_ID] >>
+  irule GENLIST_CONG >>
+  simp[subst_db_def]
 QED
 
 (* `entail` is equivalent to `full_entail`
@@ -1289,64 +1504,216 @@ QED
 * `entail`s (s,t) for all super class s of c *)
 Definition entail_wf_def:
   entail_wf cl_map inst_map ⇔
-  ∀c inst instl t clinfo s.
-    lookup inst_map c = SOME instl ∧ MEM (t,inst) instl ∧
+  ∀c tcons inst clinfo s.
+    lookup inst_map (c,tcons) = SOME inst ∧
     FLOOKUP cl_map c = SOME clinfo ∧ MEM s clinfo.super ⇒
-    entail cl_map inst_map (MAP (I ## TypeVar) inst.cstr) (s,t)
+    ∃inst'. lookup inst_map (s,tcons) = SOME inst' ∧
+    inst'.nargs = inst.nargs ∧
+    ∀cl v. MEM (cl,v) inst'.cstr ⇒
+      MEM (cl,v) inst.cstr ∨
+      ∃scl. MEM (scl,v) inst.cstr ∧ super_reachable cl_map scl cl
 End
 
-Theorem entail_wf_super:
-  entail_wf cl_map inst_map ⇒
+Theorem entail_super_TypeVar:
+  well_scoped_inst_map inst_map ∧
+  lookup inst_map (c,tcons) = SOME inst ∧
   FLOOKUP cl_map c = SOME clinfo ∧
-  MEM s clinfo.super ∧
-  entail cl_map inst_map ps (c,t) ⇒
-  entail cl_map inst_map ps (s,t)
+  MEM s clinfo.super ⇒
+  (entail cl_map inst_map (MAP (I ## TypeVar) inst.cstr)
+    (s,tcons_to_type tcons (GENLIST TypeVar inst.nargs)) ⇔
+   ∃inst'. lookup inst_map (s,tcons) = SOME inst' ∧
+    inst'.nargs = inst.nargs ∧
+    ∀cl v. MEM (cl,v) inst'.cstr ⇒
+      MEM (cl,v) inst.cstr ∨
+      ∃scl. MEM (scl,v) inst.cstr ∧ super_reachable cl_map scl cl)
 Proof
-  rw[] >>
-  pop_assum $ strip_assume_tac o SRULE[Once entail_cases]
+  rw[EQ_IMP_THM]
   >- (
-    irule entail_super >>
-    first_assum $ irule_at (Pos hd) >>
-    simp[super_reachable_def] >>
-    irule TC_SUBSET >>
-    simp[]
-  )
-  >- (
-    irule entail_super >>
-    first_assum $ irule_at (Pos hd) >>
-    fs[super_reachable_def] >>
-    irule TC_RIGHT1_I >>
-    first_assum $ irule_at (Pos last) >>
-    simp[]
-  )
-  >- (
-    drule by_inst_SOME >>
-    rw[] >>
-    fs[entail_wf_def] >>
-    last_x_assum drule >>
-    disch_then $ drule_at_then (Pos last) (drule_at (Pos last)) >>
-    disch_then $ qspecl_then
-      [`SND (EL i instl)`,`FST (EL i instl)`] mp_tac >>
-    impl_tac
+    reverse $ pop_assum $ strip_assume_tac o SRULE[Once entail_cases]
     >- (
-      rw[MEM_EL]  >>
-      metis_tac[]
+      gvs[by_inst_lem,split_ty_head_tcons_to_type,MEM_MAP,PULL_EXISTS] >>
+      rw[] >>
+      `v < inst_info.nargs` by (
+        gvs[well_scoped_inst_map_def] >>
+        last_x_assum irule >>
+        metis_tac[MEM_EL]) >>
+      first_x_assum drule >>
+      rw[Once entail_cases] >>
+      gvs[MEM_MAP]
+      >- (
+        rename1 `MEM p inst.cstr` >>
+        Cases_on `p` >>
+        gvs[]
+      )
+      >- (
+        rename1 `MEM p inst.cstr` >>
+        Cases_on `p` >>
+        gvs[] >>
+        disj2_tac >>
+        metis_tac[]
+      ) >>
+      gvs[by_inst_lem,split_ty_head_thm,head_ty_cons_def]
     ) >>
-    gvs[] >>
-  )
+    gvs[MEM_MAP] >>
+    rename1 `MEM p inst.cstr` >>
+    Cases_on `p` >>
+    gvs[tcons_to_type_NEQ_TypeVar]
+  ) >>
+  irule entail_inst >>
+  rw[by_inst_lem,split_ty_head_tcons_to_type,MEM_MAP,PULL_EXISTS] >>
+  rename1 `entail _ _ _ (_ p)` >>
+  Cases_on `p` >>
+  first_x_assum drule >>
+  rw[]
+  >- (
+    irule entail_mem >>
+    simp[MEM_MAP] >>
+    first_assum $ irule_at (Pos last) >>
+    DEP_REWRITE_TAC[EL_GENLIST] >>
+    gvs[well_scoped_inst_map_def] >>
+    last_x_assum irule >>
+    metis_tac[MEM_EL]
+  ) >>
+  irule entail_super >>
+  simp[MEM_MAP] >>
+  first_assum $ irule_at (Pos last) >>
+  first_assum $ irule_at (Pos last) >>
+  simp[] >>
+  DEP_REWRITE_TAC[EL_GENLIST] >>
+  gvs[well_scoped_inst_map_def] >>
+  last_x_assum irule >>
+  metis_tac[MEM_EL]
 QED
 
-Theorem entail_wf_super_reachable:
+Theorem entail_wf_alt:
+  well_scoped_inst_map inst_map ⇒
+  (entail_wf cl_map inst_map ⇔
+  ∀c tcons inst clinfo s.
+    lookup inst_map (c,tcons) = SOME inst ∧
+    FLOOKUP cl_map c = SOME clinfo ∧ MEM s clinfo.super ⇒
+    entail cl_map inst_map (MAP (I ## TypeVar) inst.cstr)
+      (s,tcons_to_type tcons (GENLIST TypeVar inst.nargs)))
+Proof
+  rw[entail_wf_def,EQ_IMP_THM]
+  >- (
+    first_x_assum $ drule_then $ drule_then drule >>
+    rw[] >>
+    metis_tac[entail_super_TypeVar]
+  ) >>
+  first_x_assum $ drule_then $ drule_then drule >>
+  metis_tac[entail_super_TypeVar]
+QED
+
+Triviality entail_wf_lookup_super:
+  entail_wf cl_map inst_map ∧
+  FLOOKUP cl_map c = SOME c' ∧
+  MEM s c'.super ∧
+  lookup inst_map (c,tcons) = SOME inst ⇒
+  ∃inst'. lookup inst_map (s,tcons) = SOME inst' ∧
+    inst'.nargs = inst.nargs ∧
+    ∀cl v. MEM (cl,v) inst'.cstr ⇒
+      MEM (cl,v) inst.cstr ∨
+      ∃scl. MEM (scl,v) inst.cstr ∧ super_reachable cl_map scl cl
+Proof
+  rw[] >>
+  gvs[entail_wf_def] >>
+  ntac 2 (first_x_assum drule >> rw[]) >>
+  gvs[]
+QED
+
+Theorem entail_wf_lookup_super_reachable:
   entail_wf cl_map inst_map ⇒
   ∀c s. super_reachable cl_map c s ⇒
-    entail cl_map inst_map ps (c,t) ⇒
+  ∀tcons inst. lookup inst_map (c,tcons) = SOME inst ⇒
+  ∃inst'. lookup inst_map (s,tcons) = SOME inst' ∧
+    inst'.nargs = inst.nargs ∧
+    ∀cl v. MEM (cl,v) inst'.cstr ⇒
+      MEM (cl,v) inst.cstr ∨
+      ∃scl. MEM (scl,v) inst.cstr ∧ super_reachable cl_map scl cl
+Proof
+  strip_tac >>
+  simp[Once super_reachable_def] >>
+  ho_match_mp_tac TC_INDUCT_LEFT1 >>
+  rw[]
+  >- metis_tac[entail_wf_lookup_super] >>
+  drule_all entail_wf_lookup_super >>
+  rw[] >>
+  last_x_assum drule >> rw[] >>
+  rw[] >>
+  first_x_assum drule >> rw[] >>
+  first_x_assum drule >> rw[]
+  >- metis_tac[] >>
+  disj2_tac >>
+  irule_at (Pos last) super_reachable_trans >>
+  metis_tac[]
+QED
+
+Theorem entail_strong_ind:
+  ∀cl_map inst_map ps entail'.
+    (∀p. MEM p ps ⇒ entail' p) ∧
+    (∀c s t.
+      MEM (c,t) ps ∧ super_reachable cl_map c s ⇒ entail' (s,t)) ∧
+    (∀c qs t.
+      by_inst inst_map c t = SOME qs ∧ (∀q. MEM q qs ⇒
+        entail cl_map inst_map ps q ∧ entail' q) ⇒
+      entail' (c,t)) ⇒
+  ∀a0. entail cl_map inst_map ps a0 ⇒ entail' a0
+Proof
+  rpt gen_tac >>
+  strip_tac >>
+  `∀a0. entail cl_map inst_map ps a0 ⇒
+    entail' a0 ∧ entail cl_map inst_map ps a0` suffices_by rw[] >>
+  ho_match_mp_tac entail_ind >>
+  rw[]
+  >- drule_all_then irule entail_mem
+  >- metis_tac[]
+  >- drule_all_then irule entail_super >>
+  irule entail_inst >>
+  rw[]
+QED
+
+Triviality entail_wf_super_reachable':
+  entail_wf cl_map inst_map ⇒
+  ∀p. entail cl_map inst_map ps p ⇒
+    ∀c t clinfo s. p = (c,t) ∧
+    (c = s ∨
+    super_reachable cl_map c s) ⇒
     entail cl_map inst_map ps (s,t)
 Proof
   strip_tac >>
-  simp[super_reachable_def] >>
-  ho_match_mp_tac TC_INDUCT_LEFT1 >>
+  ho_match_mp_tac entail_strong_ind >>
+  rw[]
+  >- drule_then irule entail_mem
+  >- drule_all_then irule entail_super
+  >- drule_all_then irule entail_super
+  >- (
+    irule entail_super >>
+    first_assum $ irule_at (Pos hd) >>
+    drule_all_then irule super_reachable_trans) >>
+  gvs[IMP_CONJ_THM,FORALL_AND_THM] >>
+  gvs[PULL_FORALL,AND_IMP_INTRO]
+  >- drule_all_then irule entail_inst >>
+  gvs[by_inst_lem,MEM_MAP,PULL_EXISTS,LAMBDA_PROD,
+    GSYM PFORALL_THM,GSYM PEXISTS_THM] >>
+  irule entail_inst >>
+  simp[by_inst_lem,MEM_MAP,
+    PULL_EXISTS,LAMBDA_PROD,GSYM PFORALL_THM] >>
+  drule_all entail_wf_lookup_super_reachable >>
   rw[] >>
-  metis_tac[entail_wf_super]
+  rw[MEM_MAP,GSYM PEXISTS_THM] >>
+  first_x_assum drule >>
+  rw[] >>
+  first_x_assum drule >> rw[]
+QED
+
+Theorem entail_wf_super_reachable:
+  ∀cl_map inst_map ps c t s.
+    entail_wf cl_map inst_map ∧
+    entail cl_map inst_map ps (c,t) ∧
+    super_reachable cl_map c s ⇒
+    entail cl_map inst_map ps (s,t)
+Proof
+  metis_tac[entail_wf_super_reachable']
 QED
 
 Theorem entail_eq_full_entail:
@@ -1373,40 +1740,106 @@ Proof
   >- drule_all_then irule entail_inst
 QED
 
-Definition entail_terminate_wf_def:
-  entail_terminate_wf inst_map ⇔
-  ∀c instl t inst.
-    lookup inst_map c = SOME instl ∧
-    MEM (t,inst) instl ∧
-    (∀x. t ≠ TypeVar x)
-End
+Theorem entail_monotone:
+  ∀p. entail cl_map inst_map ps p ⇒
+  (∀q. MEM q ps ⇒ MEM q qs) ⇒
+  entail cl_map inst_map qs p
+Proof
+  ho_match_mp_tac entail_ind >>
+  rw[]
+  >- (irule entail_mem >> metis_tac[])
+  >- (irule entail_super >> metis_tac[]) >>
+  irule entail_inst >> metis_tac[]
+QED
 
-Definition inst_map_scoped_def:
-  inst_map_scoped inst_map ⇔
-  ∀c instl t inst.
-    lookup inst_map c = SOME instl ∧
-    MEM (t,inst) instl ∧
-    (∀c' v. MEM (c',v) inst.cstr ⇒ scoped c t)
-End
+Theorem full_entail_monotone:
+  ∀p. full_entail cl_map inst_map ps p ⇒
+  (∀q. MEM q ps ⇒ MEM q qs) ⇒
+  full_entail cl_map inst_map qs p
+Proof
+  ho_match_mp_tac full_entail_ind >>
+  rw[]
+  >- (irule full_entail_mem >> metis_tac[])
+  >- (irule full_entail_super >> metis_tac[]) >>
+  irule full_entail_inst >> metis_tac[]
+QED
+
+Theorem full_entail_add_full_entail:
+  ∀p. full_entail cl_map inst_map (q::ps) p ⇒
+  full_entail cl_map inst_map ps q ⇒
+  full_entail cl_map inst_map ps p
+Proof
+  ho_match_mp_tac full_entail_ind >>
+  rw[]
+  >- simp[]
+  >- drule_then irule full_entail_mem
+  >- (irule full_entail_super >> metis_tac[]) >>
+  drule_then irule full_entail_inst >>
+  rw[]
+QED
+
+Triviality type_size_GT_0:
+  ∀t. 0 < type_size t
+Proof
+  Cases_on `t` >>
+  simp[type_size_def]
+QED
+
+Theorem type_size_tcons_to_type:
+  ∀t targs.
+  MEM t targs ⇒
+  type_size t < type_size (tcons_to_type tcons targs)
+Proof
+  Induct_on `targs` using SNOC_INDUCT >>
+  rw[tcons_to_type_SNOC,type_size_def]
+  >- rw[] >>
+  irule arithmeticTheory.LESS_TRANS >>
+  first_x_assum $ drule_then $ irule_at (Pos hd) >>
+  DECIDE_TAC
+QED
 
 (* entail_aux terminates if every q in qs is smaller than t *)
 Definition entail_aux_def:
   (entail_aux supers inst_map (c,t) =
-    if entail_terminate_wf inst_map
+    if well_scoped_inst_map inst_map
     then
-      EXISTS (\visited. lookup visited c = SOME t) supers ∨
+      (EXISTS (\visited. lookup visited c = SOME t) supers ∨
       (case by_inst inst_map c t of
         | NONE => F
-        | SOME qs => entail_aux_list supers inst_map qs)
-     else F (* should never happen *)) ∧
-  ((entail_aux_list supers inst_map [] = T) ∧
+        | SOME qs => entail_aux_list supers inst_map qs))
+    else F (* should not happen given the map is well formed *)) ∧
+
+  (entail_aux_list supers inst_map [] = T) ∧
   (entail_aux_list supers inst_map (q::qs) =
-    (entail_aux supers inst_map q) ∧
+    (entail_aux supers inst_map q ∧
      entail_aux_list supers inst_map qs))
 Termination
-  (* LENGTH LEX type_size *)
-  WF_REL_TAC `_ LEX _` >>
-  cheat
+  WF_REL_TAC `inv_image ($< LEX $<) (λx.
+    (case x of
+     | INR (_,_,qs) => list_max $ MAP (type_size o SND) qs
+     | INL (_,_,_,t) => type_size t),
+    (case x of
+     | INR (_,_,qs) => LENGTH qs
+     | INL _ => 0))` >>
+  rw[]
+  >- (
+    gvs[by_inst_lem] >>
+    PURE_REWRITE_TAC[Once $ GSYM arithmeticTheory.GREATER_DEF] >>
+    irule list_max_intro >>
+    simp[EVERY_MAP,arithmeticTheory.GREATER_DEF,type_size_GT_0] >>
+    drule_then (assume_tac o GSYM) tcons_to_type_split_ty_head >>
+    gvs[EVERY_EL] >>
+    rw[] >>
+    gvs[well_scoped_inst_map_def] >>
+    last_x_assum $ drule_then strip_assume_tac >>
+    irule type_size_tcons_to_type >>
+    Cases_on `EL n inst_info.cstr` >>
+    gvs[] >>
+    rename1 `EL n inst_info.cstr = (a,b)` >>
+    first_x_assum $ qspecl_then [`a`,`b`] mp_tac >>
+    metis_tac[MEM_EL]
+  ) >>
+  simp[GSYM arithmeticTheory.LE_LT,list_max_def]
 End
 
 Definition entail_impl_def:
@@ -1415,6 +1848,122 @@ Definition entail_impl_def:
    | NONE => F
    | SOME visiteds => entail_aux visiteds inst_map (c,t)
 End
-*)
+
+Theorem entail_aux_list_EVERY:
+  entail_aux_list supers inst_map = EVERY (entail_aux supers inst_map)
+Proof
+  rw[FUN_EQ_THM] >>
+  rename1 `entail_aux_list _ _ l` >>
+  Induct_on `l` >>
+  simp[entail_aux_def]
+QED
+
+Theorem entail_aux_induct_EVERY:
+  ∀P.
+  (∀(supers:(mlstring,type) map list) inst_map c t.
+    (∀qs q.
+      well_scoped_inst_map inst_map ∧
+      by_inst inst_map c t = SOME qs ∧ MEM q qs ⇒
+      P supers inst_map q) ⇒
+    P supers inst_map (c,t)) ⇒
+    (∀supers inst_map p. P supers inst_map p)
+Proof
+  ntac 2 strip_tac >>
+  qspecl_then [`P`,`λv0 v1 v2. ∀q. MEM q v2 ⇒ P v0 v1 q`]
+    mp_tac entail_aux_ind >>
+  impl_tac >>
+  rw[] >>
+  metis_tac[]
+QED
+
+Theorem OPT_MMAP_SOME_EL:
+  ∀l fl. OPT_MMAP f l = SOME fl ⇒
+  LENGTH fl = LENGTH l ∧
+  (∀n. n < LENGTH l ⇒ f (EL n l) = SOME (EL n fl))
+Proof
+  Induct_on `l` >>
+  rw[OPT_MMAP_def] >>
+  gvs[] >>
+  Cases_on `n` >>
+  simp[]
+QED
+
+Theorem OPT_MMAP_NONE:
+  ∀l. OPT_MMAP f l = NONE ⇒
+  ∃x. MEM x l ∧ f x = NONE
+Proof
+  Induct_on `l` >>
+  rw[OPT_MMAP_def] >>
+  metis_tac[]
+QED
+
+Theorem entail_aux_thm:
+  ∀supers inst_map p cl_map ps.
+  map_ok cl_map ∧ map_ok inst_map ∧
+  well_scoped_inst_map inst_map ∧ super_keys_ok cl_map ∧
+  (∀q. MEM q ps ⇒ ∃clinfo. lookup cl_map (FST q) = SOME clinfo) ∧
+  (LENGTH supers = LENGTH ps) ∧
+  (∀n. n < LENGTH ps ⇒
+    by_super cl_map (EL n ps) = SOME (EL n supers)) ⇒
+  (entail_aux supers inst_map p ⇔
+    entail (to_class_map cl_map) inst_map ps p)
+Proof
+  ho_match_mp_tac entail_aux_induct_EVERY >>
+  rw[] >>
+  gvs[AND_IMP_INTRO,cj 1 PULL_FORALL] >>
+  last_x_assum $ drule_at (Pos last) >>
+  rw[] >>
+  simp[entail_aux_def] >>
+  rw[EQ_IMP_THM]
+  >- (
+    gvs[EXISTS_MEM] >>
+    qpat_x_assum `MEM visited supers` $
+      strip_assume_tac o SRULE[MEM_EL] >>
+    gvs[] >>
+    first_x_assum $ drule_then assume_tac >>
+    Cases_on `EL n ps` >>
+    drule_all $ iffLR by_super_thm >>
+    rw[]
+    >- (irule entail_mem >> metis_tac[MEM_EL]) >>
+    irule entail_super >> metis_tac[MEM_EL]
+  )
+  >- (
+    pop_assum mp_tac >>
+    TOP_CASE_TAC >>
+    rw[entail_aux_list_EVERY,EVERY_MEM] >>
+    irule entail_inst >>
+    simp[]
+  ) >>
+  reverse $ pop_assum $ strip_assume_tac o SRULE[Once entail_cases]
+  >- simp[entail_aux_list_EVERY,EVERY_MEM] >>
+  qpat_x_assum `MEM _ ps` $
+    strip_assume_tac o GSYM o SRULE[MEM_EL] >>
+  first_x_assum $ drule_then assume_tac >>
+  gvs[EXISTS_MEM] >>
+  drule_then strip_assume_tac $
+    SRULE[DISJ_IMP_THM,FORALL_AND_THM] $ iffRL by_super_thm >>
+  metis_tac[MEM_EL]
+QED
+
+Theorem entail_impl_thm:
+  map_ok cl_map ∧ map_ok inst_map ∧
+  well_scoped_inst_map inst_map ∧ super_keys_ok cl_map ∧
+  (∀q. MEM q ps ⇒ ∃clinfo. lookup cl_map (FST q) = SOME clinfo) ⇒
+  entail_impl cl_map inst_map ps p =
+    entail (to_class_map cl_map) inst_map ps p
+Proof
+  rw[oneline entail_impl_def] >>
+  ntac 2 TOP_CASE_TAC
+  >- (
+    dxrule_then strip_assume_tac OPT_MMAP_NONE >>
+    first_assum $ drule_then strip_assume_tac >>
+    drule_all_then (qspec_then `SND x` mp_tac) $
+      SRULE[PULL_EXISTS] $ iffLR well_formed_by_super >>
+    rw[]
+  ) >>
+  dxrule_then strip_assume_tac OPT_MMAP_SOME_EL >>
+  irule entail_aux_thm >>
+  rw[]
+QED
 
 val _ = export_theory();
